Finite.v
@@ -1,0 +1,173 @@
+From Equations Require Import Equations.
+Require Import Coq.Lists.List.
+Require Import Coq.Program.Equality.
+
+Class Finite (X: Type) := {
+  finite_enum: list X;
+  finite_dec: forall (x1 x2: X), {x1 = x2} + {x1 <> x2};
+  finite_eqb x1 x2 := if finite_dec x1 x2 then true else false;
+  finite_cover: forall x, In x finite_enum;
+  finite_nodup: NoDup finite_enum;
+}.
+
+Inductive position: nat -> Type :=
+| PHere:
+    forall {n: nat},
+    position (S n)
+| PThere:
+    forall {n: nat}
+           (v: position n),
+    position (S n)
+.
+
+Section FiniteIsomorphism.
+  Equations list_lookup_helper
+    {X: Type}
+    (l: list X)
+    (n: position (length l))
+    : X
+  := {
+    list_lookup_helper (x :: _) PHere := x;
+    list_lookup_helper (_ :: l) (PThere p) := list_lookup_helper l p;
+  }.
+
+  Definition list_lookup
+    {X: Type}
+    `{Finite X}
+    (n: position (length finite_enum))
+    : X
+  :=
+    list_lookup_helper finite_enum n
+  .
+
+  Equations list_index_helper
+    {X: Type}
+    (l: list X)
+    (x: X)
+    (Hdec: forall (x1 x2: X), {x1 = x2} + {x1 <> x2})
+    (Hin: In x l)
+    : position (length l)
+  :=
+    list_index_helper (x' :: l) x Hdec Hin :=
+      if Hdec x' x then PHere
+      else PThere (list_index_helper l x Hdec _)
+  .
+  Next Obligation.
+    now destruct Hin.
+  Defined.
+
+  Definition list_index
+    {X: Type}
+    `{Finite X}
+    (x: X)
+    : position (length finite_enum)
+  :=
+    list_index_helper finite_enum x finite_dec (finite_cover x)
+  .
+
+  Lemma list_lookup_helper_in
+    {X: Type}
+    (l: list X)
+    (p: position (length l))
+  :
+    In (list_lookup_helper l p) l
+  .
+  Proof.
+    induction l.
+    - dependent destruction p.
+    - dependent destruction p.
+      + autorewrite with list_lookup_helper.
+        now left.
+      + autorewrite with list_lookup_helper.
+        right.
+        apply IHl.
+  Qed.
+
+  Lemma list_lookup_helper_injective
+    {X: Type}
+    (l: list X)
+    (p1 p2: position (length l))
+  :
+    NoDup l ->
+    list_lookup_helper l p1 = list_lookup_helper l p2 ->
+    p1 = p2
+  .
+  Proof.
+    induction l; intros.
+    - dependent destruction p1.
+    - dependent destruction p1;
+      dependent destruction p2;
+      autorewrite with list_lookup_helper in H0;
+      auto.
+      + exfalso.
+        pose proof (list_lookup_helper_in l p2).
+        rewrite <- H0 in H1.
+        now inversion H.
+      + exfalso.
+        pose proof (list_lookup_helper_in l p1).
+        rewrite H0 in H1.
+        now inversion H.
+      + autorewrite with list_lookup_helper in H0.
+        f_equal.
+        apply IHl; auto.
+        now inversion H.
+  Qed.
+
+  Lemma list_lookup_injective
+    {X: Type}
+    `{Finite X}
+    (p1 p2: position (length finite_enum))
+  :
+    list_lookup p1 = list_lookup p2 ->
+    p1 = p2
+  .
+  Proof.
+    unfold list_lookup; intros.
+    apply list_lookup_helper_injective; auto.
+    apply finite_nodup.
+  Qed.
+
+  Lemma list_lookup_helper_list_index_helper
+    {X: Type}
+    (l: list X)
+    (x: X)
+    (Hdec: forall (x x': X), {x = x'} + {x <> x'})
+    (Hin: In x l)
+  :
+    list_lookup_helper l (list_index_helper l x Hdec Hin) = x
+  .
+  Proof.
+    induction l.
+    - destruct Hin.
+    - autorewrite with list_index_helper.
+      destruct (Hdec a x);
+      autorewrite with list_lookup_helper.
+      + assumption.
+      + now rewrite IHl.
+  Qed.
+
+  Lemma list_lookup_index
+    {X: Type}
+    `{Finite X}
+    (x: X)
+  :
+    list_lookup (list_index x) = x
+  .
+  Proof.
+    unfold list_lookup.
+    unfold list_index.
+    apply list_lookup_helper_list_index_helper.
+  Qed.
+
+  Lemma list_index_lookup
+    {X: Type}
+    `{Finite X}
+    (p: position (length finite_enum))
+  :
+    list_index (list_lookup p) = p
+  .
+  Proof.
+    apply list_lookup_injective.
+    now rewrite list_lookup_index.
+  Qed.
+End FiniteIsomorphism.
